convert to Utf8 and cleaner Notations

theories/beta.v
@@ -7,7 +7,7 @@
 (*        Mozilla Public License Version 2.0, MPL-2.0         *)
 (**************************************************************)
 
-From Coq Require Import List Relations Wellfounded.
+From Coq Require Import List Relations Wellfounded Utf8.
 Import ListNotations.
 
 From SystemF Require Import utils syntax.
@@ -21,29 +21,29 @@ Set Implicit Arguments.
 #[global] Reserved Notation "x '-β*>' y" (at level 70).
 
 Inductive term_beta : term -> term -> Prop :=
-  | in_beta_redex u v :         (λ u)@v -β-> u⌈v⌉
+  | in_beta_redex u v :         (Ⲗ u)@v -β-> u⌈v⌉
   | in_beta_lft u v w : u -β-> v -> u@w -β-> v@w
   | in_beta_rt  u v w : u -β-> v -> w@u -β-> w@v
-  | in_beta_abs u v   : u -β-> v -> λ u -β-> λ v
+  | in_beta_abs u v   : u -β-> v -> Ⲗ u -β-> Ⲗ v
 where  "x -β-> y" := (@term_beta x y).
 
 #[global] Hint Constructors term_beta : core.
 
 #[local] Hint Resolve in_or_app in_app_or list_pred_mono syn_replace_vars : core.
 
-Fact term_beta_vars u v : u -β-> v -> incl (syn_vars v) (syn_vars u).
+Fact term_beta_vars u v : u -β-> v → incl (𝓥 v) (𝓥 u).
 Proof. unfold incl; induction 1; simpl; eauto; intros ? []%in_app_or; auto. Qed.
 
 (*
 Inductive term_beta_inv_abs u : term -> Prop :=
-  | in_term_beta_inv_abs_0 v : u -β-> v -> term_beta_inv_abs u (λ v).
+  | in_term_beta_inv_abs_0 v : u -β-> v -> term_beta_inv_abs u (Ⲗ v).
 
 Inductive term_beta_inv_app v : term -> term -> Prop :=
   | in_term_beta_inv_app_0 u u' : u -β-> u' -> term_beta_inv_app v u (u'@v)
   | in_term_beta_inv_app_1 v
 *)
 
-Fact term_beta_app u v l : u -β-> v -> u @* l -β-> v @* l.
+Fact term_beta_app u v l : u -β-> v → u @* l -β-> v @* l.
 Proof.
   intros.
   induction l using list_snoc_rect; auto.
@@ -52,66 +52,64 @@ Qed.
 
 #[local] Hint Resolve term_beta_app : core.
 
-Fact term_beta_app_middle a l u v r : u -β-> v -> a @* l++u::r -β-> a @* l++v::r.
+Fact term_beta_app_middle a l u v r : u -β-> v → a @* l++u::r -β-> a @* l++v::r.
 Proof. intro; rewrite !term_app_comp; simpl; auto. Qed.
 
 Notation "x -β+> y" := (clos_trans term_beta x y).
 Notation "x -β*> y" := (clos_refl_trans term_beta x y).
 
-Fact term_betastar_vars u v : u -β*> v -> incl (syn_vars v) (syn_vars u).
+Fact term_betastar_vars u v : u -β*> v → incl (𝓥 v) (𝓥 u).
 Proof. unfold incl; induction 1; eauto; now apply term_beta_vars. Qed. 
 
-Fact term_betaplus_abs u v : u -β+> v -> λ u -β+> λ v.
+Fact term_betaplus_abs u v : u -β+> v → Ⲗ u -β+> Ⲗ v.
 Proof. apply clos_trans_fun; eauto. Qed.
 
-Fact term_betastar_abs u v : u -β*> v -> λ u -β*> λ v.
+Fact term_betastar_abs u v : u -β*> v → Ⲗ u -β*> Ⲗ v.
 Proof. apply clos_refl_trans_fun; eauto. Qed.
 
-Fact term_betaplus_lft u v w : u -β+> v -> u@w -β+> v@w.
+Fact term_betaplus_lft u v w : u -β+> v → u@w -β+> v@w.
 Proof. apply clos_trans_fun with (f := fun u => u@w); eauto. Qed.
 
-Fact term_betastar_lft u v w : u -β*> v -> u@w -β*> v@w.
+Fact term_betastar_lft u v w : u -β*> v → u@w -β*> v@w.
 Proof. apply clos_refl_trans_fun with (f := fun u => u@w); eauto. Qed.
 
-Fact term_betaplus_rt u v w : v -β+> w -> u@v -β+> u@w.
+Fact term_betaplus_rt u v w : v -β+> w → u@v -β+> u@w.
 Proof. apply clos_trans_fun with (f := fun w => u@w); eauto. Qed.
 
-Fact term_betastar_rt u v w : v -β*> w -> u@v -β*> u@w.
+Fact term_betastar_rt u v w : v -β*> w → u@v -β*> u@w.
 Proof. apply clos_refl_trans_fun with (f := fun w => u@w); eauto. Qed.
 
-Fact term_betastar_app u v l : u -β*> v -> u @* l -β*> v @* l.
+Fact term_betastar_app u v l : u -β*> v → u @* l -β*> v @* l.
 Proof. apply clos_refl_trans_fun with (f := fun u => u @* l); eauto. Qed.
 
 #[local] Hint Resolve term_betastar_lft term_betastar_rt : core.
 
-Fact term_beta_ren u v f : u -β-> v -> syn_ren u f -β-> syn_ren v f.
+Fact term_beta_ren u v f : u -β-> v → u⟬f⟭ -β-> v⟬f⟭.
 Proof.
   induction 1 in f |- *; simpl; eauto.
   rewrite syn_ren_replace; constructor.
 Qed.
 
-Fact term_beta_lift u v : u -β-> v -> ↑u -β-> ↑v.
+Fact term_beta_lift u v : u -β-> v → ↑u -β-> ↑v.
 Proof. apply term_beta_ren. Qed.
 
 #[local] Hint Resolve term_beta_ren term_beta_lift : core.
 
-Fact term_betastar_ren u v f : u -β*> v -> syn_ren u f -β*> syn_ren v f.
+Fact term_betastar_ren u v f : u -β*> v → u⟬f⟭ -β*> v⟬f⟭.
 Proof. apply clos_refl_trans_fun with (f := fun u => syn_ren u f); auto. Qed.
 
-Fact term_beta_subst u v f : u -β-> v -> syn_subst u f -β-> syn_subst v f.
+Fact term_beta_subst u v f : u -β-> v → u⟪f⟫ -β-> v⟪f⟫.
 Proof.
   induction 1 in f |- *; simpl; eauto.
   rewrite syn_subst_replace; eauto.
 Qed.
 
-Fact term_beta_replace u v a : u -β-> v -> u⌈a⌉ -β-> v⌈a⌉.
+Fact term_beta_replace u v a : u -β-> v → u⌈a⌉ -β-> v⌈a⌉.
 Proof. apply term_beta_subst. Qed.
 
 #[local] Hint Resolve in_or_app in_eq in_cons : core.
 
-Lemma term_betastar_subst u f g :
-        (forall x, x ∈ syn_vars u -> f x -β*> g x)
-     -> syn_subst u f -β*> syn_subst u g.
+Lemma term_betastar_subst u f g : (∀x, x ∈ 𝓥 u → f x -β*> g x) → u⟪f⟫ -β*> u⟪g⟫.
 Proof.
   induction u as [ x | u IHu v IHv | u IHu ] in f, g |- *; simpl; intros H; eauto.
   + constructor 3 with (syn_subst u f@syn_subst v g).
@@ -128,16 +126,14 @@ Qed.
     DO NOT HOLD because u might no contain
     any occurence of the variable 0 and hence,
     there would be no reduction because u⌈a⌉ = u⌈b⌉ = u⌈_⌉ *)
-Lemma term_betastar_replace u a b : a -β*> b -> u⌈a⌉ -β*> u⌈b⌉.
+Lemma term_betastar_replace u a b : a -β*> b → u⌈a⌉ -β*> u⌈b⌉.
 Proof.
   intro; apply term_betastar_subst.
   intros []; simpl; eauto.
 Qed.
 
 Local Fact term_beta_ren_inv_rec u v :
-        u -β-> v
-     -> forall f u', u = syn_ren u' f 
-     -> exists v', v = syn_ren v' f /\ u' -β-> v'.
+        u -β-> v → ∀ f u', u = u'⟬f⟭ → ∃v', v = v'⟬f⟭ ∧ u' -β-> v'.
 Proof.
   induction 1 as [ u v | u v w _ IH | u v w _ IH | u v _ IH ]; intros f u' E.
   + apply syn_ren_bin_eq_inv in E as (u'' & v' & -> & 
@@ -154,58 +150,73 @@ Proof.
     exists (w'@v'); eauto.
   + apply syn_ren_abs_eq_inv in E as (u'' & -> & ->).
     destruct (IH _ _ eq_refl) as (v' & -> & ?).
-    exists (λ v'); eauto.
+    exists (Ⲗ v'); eauto.
 Qed.
 
-Fact term_beta_ren_inv u f w :
-        syn_ren u f -β-> w
-     -> exists v, w = syn_ren v f /\ u -β-> v.
+Fact term_beta_ren_inv u f w : u⟬f⟭ -β-> w → ∃v, w = v⟬f⟭ ∧ u -β-> v.
 Proof. intros H; apply term_beta_ren_inv_rec with (2 := eq_refl) in H; auto. Qed.
 
-Fact term_beta_lift_inv u w : ↑u -β-> w -> exists v, w = ↑v  /\ u -β-> v.
+Fact term_beta_lift_inv u w : ↑u -β-> w → ∃v, w = ↑v ∧ u -β-> v.
 Proof. apply term_beta_ren_inv. Qed.
+
+(* A more direct proof but that will not work for arbitrary (non-injective) renaming *)
+Fact term_beta_lift_inv' u w : ↑u -β-> w → ∃v, w = ↑v ∧ u -β-> v.
+Proof.
+  intros H.
+  assert (~ In 0 (syn_vars w)) as Hv.
+  1:{ intros C%(term_beta_vars H).
+      rewrite syn_lift_vars, in_map_iff in C. 
+      now destruct C as (? & ? & _). }
+  apply (syn_replace_lift _ (£0)) in Hv.
+  rewrite <- Hv in H |- *.
+  exists (w⌈£0⌉); split; auto.
+  apply term_beta_ren with (f := pred) in H.
+  unfold syn_lift in H.
+  rewrite !syn_ren_comp in H; simpl in H.
+  now rewrite !syn_ren_id in H.
+Qed.
 
 (** We study inversions shapes for t -β-> _ *)
 
 Fact term_beta_inv u w :
     u -β-> w 
- -> match u with
+  → match u with
     | £ _  => False
-    | λ u  => exists v, w = λ v /\ u -β-> v
-    | u@v  => (exists u', w = u'@v /\ u -β-> u')
-           \/ (exists v', w = u@v' /\ v -β-> v')
-           \/ (exists u', u = λ u' /\ w = u'⌈v⌉) 
+    | Ⲗ u  =>   ∃v, w = Ⲗ v ∧ u -β-> v
+    | u@v  => (∃u', w = u'@v ∧ u -β-> u')
+            ∨ (∃v', w = u@v' ∧ v -β-> v')
+            ∨ (∃u', u = Ⲗ u' ∧ w = u'⌈v⌉) 
     end. 
 Proof. intros []; simpl; eauto. Qed.
 
 (*
 
 Inductive term_beta_lam_invt : term -> term -> Prop :=
-  | term_beta_lam_invt0 u v : u -β-> v -> term_beta_lam_invt (λ u) (λ v).
+  | term_beta_lam_invt0 u v : u -β-> v -> term_beta_lam_invt (Ⲗ u) (Ⲗ v).
 
 Inductive term_beta_app_invt : term -> term -> Prop :=
   | term_beta_app_invt0 u u' v : u -β-> u' -> term_beta_app_invt (u@v) (u'@v)
   | term_beta_app_invt1 u v v' : v -β-> v' -> term_beta_app_invt (u@v) (u@v')
-  | term_beta_app_invt2 u v : term_beta_app_invt (λ u@v) (u⌈v⌉)
+  | term_beta_app_invt2 u v : term_beta_app_invt (Ⲗ u@v) (u⌈v⌉)
   .
 
 Fact term_beta_inv' u v :
     u -β-> v 
  -> match u with
     | £ _  => False
-    | λ _  => term_beta_lam_invt u v
+    | Ⲗ _  => term_beta_lam_invt u v
     | _@_  => term_beta_app_invt u v
     end. 
 Proof. intros []; simpl; constructor; auto. Qed.
 
 *)
 
-Inductive term_beta_redex_shape f a : term -> Prop :=
+Inductive term_beta_redex_shape f a : term → Prop :=
   | term_beta_redex_shape0 : term_beta_redex_shape f a (f⌈a⌉)
-  | term_beta_redex_shape1 g : f -β-> g -> term_beta_redex_shape f a (λ g @ a)
-  | term_beta_redex_shape2 b : a -β-> b -> term_beta_redex_shape f a (λ f @ b).
+  | term_beta_redex_shape1 g : f -β-> g → term_beta_redex_shape f a (Ⲗ g @ a)
+  | term_beta_redex_shape2 b : a -β-> b → term_beta_redex_shape f a (Ⲗ f @ b).
 
-Fact term_beta_redex_inv f a v : λ f @ a -β-> v -> term_beta_redex_shape f a v.
+Fact term_beta_redex_inv f a v : Ⲗ f @ a -β-> v → term_beta_redex_shape f a v.
 Proof.
   intros [ (? & -> & (g & -> & ?)%term_beta_inv) 
        | [ (? & -> & ?) | (f' & E & ->)] ]%term_beta_inv; try constructor; auto.
@@ -214,10 +225,10 @@ Qed.
 
 (*
 Fact term_beta_redex_inv' f a v :
-       λ f @ a -β-> v
+       Ⲗ f @ a -β-> v
     -> v = f⌈a⌉
-    \/ (exists g, v = λ g @ a /\ f -β-> g)
-    \/ (exists b, v = λ f @ b /\ a -β-> b).
+    \/ (exists g, v = Ⲗ g @ a /\ f -β-> g)
+    \/ (exists b, v = Ⲗ f @ b /\ a -β-> b).
 Proof.
   intros H%term_beta_redex_inv.
   destruct H; eauto.
@@ -227,21 +238,21 @@ Qed.
 (** We study the successors of _ @* _ for the following forms
      - £_ @* _
      - _@_ @* _
-     - λ_ @* []
-     - λ_ @* _::_ *)
+     - Ⲗ_ @* []
+     - Ⲗ_ @* _::_ *)
 
 Definition term_neutral (u : term) :=
   match u with 
-  | λ _ => False
+  | Ⲗ _ => False
   | _   => True
   end.
 
-Inductive term_beta_neutral_app_shape a : list term -> term -> Prop :=
-  | term_beta_neutral_app_shape0 b m : a -β-> b -> term_beta_neutral_app_shape a m (b @* m)
-  | term_beta_neutral_app_shape1 l v w r : v -β-> w -> term_beta_neutral_app_shape a (l++v::r) (a @* l++w::r).
+Inductive term_beta_neutral_app_shape a : list term → term → Prop :=
+  | term_beta_neutral_app_shape0 b m : a -β-> b → term_beta_neutral_app_shape a m (b @* m)
+  | term_beta_neutral_app_shape1 l v w r : v -β-> w → term_beta_neutral_app_shape a (l++v::r) (a @* l++w::r).
 
 (** This is a key lemma for the results below, by snoc induction on m *)
-Lemma term_beta_neutral_app_inv a u m : term_neutral a -> a @* m -β-> u -> term_beta_neutral_app_shape a m u.
+Lemma term_beta_neutral_app_inv a u m : term_neutral a → a @* m -β-> u → term_beta_neutral_app_shape a m u.
 Proof.
   induction m as [ | m b IHm ] in a, u |- * using list_snoc_rect; intros H1 H2.
   + simpl in H2; constructor 1 with (1:= H2).
@@ -260,10 +271,10 @@ Proof.
         now subst.
 Qed.
 
-Inductive term_beta_var_app_shape x : list term -> term -> Prop :=
-  | term_beta_var_app_shape0 l v w r : v -β-> w -> term_beta_var_app_shape x (l++v::r) (£x @* l++w::r).
+Inductive term_beta_var_app_shape x : list term → term → Prop :=
+  | term_beta_var_app_shape0 l v w r : v -β-> w → term_beta_var_app_shape x (l++v::r) (£x @* l++w::r).
 
-Fact term_beta_var_app_inv x m u : £x @* m -β-> u -> term_beta_var_app_shape x m u.
+Fact term_beta_var_app_inv x m u : £x @* m -β-> u → term_beta_var_app_shape x m u.
 Proof.
   intros H%term_beta_neutral_app_inv; simpl; auto.
   destruct H as [ _ _ []%term_beta_inv | ].
@@ -271,30 +282,29 @@ Proof.
 Qed.
 
 Fact term_beta_var_app_inv' x m u :
-         £x @* m -β-> u
-      -> exists l v w r, m = l++v::r /\ u = £x @* l++w::r /\ v -β-> w.
+         £x @* m -β-> u → ∃ l v w r, m = l++v::r ∧ u = £x @* l++w::r ∧ v -β-> w.
 Proof. intros [ l v w r ]%term_beta_var_app_inv; exists l, v, w, r; auto. Qed.
 
-Inductive term_beta_ap_app_shape a b : list term -> term -> Prop :=
-  | term_beta_ap_app_shape0 m t : a@b -β-> t -> term_beta_ap_app_shape a b m (t @* m)
-  | term_beta_ap_app_shape1 l v w r : v -β-> w -> term_beta_ap_app_shape a b (l++v::r) ((a@b) @* l++w::r).
+Inductive term_beta_ap_app_shape a b : list term → term → Prop :=
+  | term_beta_ap_app_shape0 m t : a@b -β-> t → term_beta_ap_app_shape a b m (t @* m)
+  | term_beta_ap_app_shape1 l v w r : v -β-> w → term_beta_ap_app_shape a b (l++v::r) ((a@b) @* l++w::r).
 
-Fact term_beta_ap_app_inv a b m u : (a@b) @* m -β-> u -> term_beta_ap_app_shape a b m u.
+Fact term_beta_ap_app_inv a b m u : (a@b) @* m -β-> u → term_beta_ap_app_shape a b m u.
 Proof.
   intros H%term_beta_neutral_app_inv; simpl; auto.
   destruct H; constructor; auto.
 Qed.
 
-Fact term_beta_lam_app0_inv a u : λ a @* [] -β-> u -> exists b, u = λ b @* [] /\ a -β-> b.
+Fact term_beta_lam_app0_inv a u : Ⲗ a @* [] -β-> u → ∃b, u = Ⲗ b @* [] ∧ a -β-> b.
 Proof. now intros H%term_beta_inv. Qed.
 
-Inductive term_beta_redex_app_shape u a : list term -> term -> Prop :=
+Inductive term_beta_redex_app_shape u a : list term → term → Prop :=
   | term_beta_redex_app_shape0 m : term_beta_redex_app_shape u a m (u⌈a⌉ @* m)
-  | term_beta_redex_app_shape1 m v : u -β-> v -> term_beta_redex_app_shape u a m (λ v @* a::m)
-  | term_beta_redex_app_shape2 m b : a -β-> b -> term_beta_redex_app_shape u a m (λ u @* b::m)
-  | term_beta_redex_app_shape3 l v w r : v -β-> w -> term_beta_redex_app_shape u a (l++v::r) (λ u @* a::l++w::r).
+  | term_beta_redex_app_shape1 m v : u -β-> v → term_beta_redex_app_shape u a m (Ⲗ v @* a::m)
+  | term_beta_redex_app_shape2 m b : a -β-> b → term_beta_redex_app_shape u a m (Ⲗ u @* b::m)
+  | term_beta_redex_app_shape3 l v w r : v -β-> w → term_beta_redex_app_shape u a (l++v::r) (Ⲗ u @* a::l++w::r).
 
-Fact term_beta_redex_app_inv u a m t : λ u @* a::m -β-> t -> term_beta_redex_app_shape u a m t.
+Fact term_beta_redex_app_inv u a m t : Ⲗ u @* a::m -β-> t → term_beta_redex_app_shape u a m t.
 Proof.
   intros H%term_beta_ap_app_inv.
   destruct H as [ m t H%term_beta_redex_inv | ].
@@ -304,24 +314,26 @@ Qed.
 
 (** We study strong normalization *)
 
+(*
 Definition term_beta_normal u := forall v, ~ u -β-> v.
 
 Fact term_var_beta_normal x : term_beta_normal (£x).
 Proof. now intros ? ?%term_beta_inv. Qed.
+*)
 
-Definition term_beta_sn := Acc (fun u v => term_beta v u).
+Definition term_beta_sn := Acc (rinv term_beta).
 
 #[local] Notation SN := term_beta_sn.
 
-Fact term_betastar_sn u v : u -β*> v -> SN u -> SN v.
+Fact term_betastar_sn u v : u -β*> v → SN u → SN v.
 Proof. apply Acc_inv_clos_refl_trans_rinv. Qed.
 
 Fact term_beta_sn_inv u :
        SN u
-    -> match u with
+     → match u with
        | £ _ => True
-       | u@v => SN u /\ SN v
-       | λ u => SN u
+       | u@v => SN u ∧ SN v
+       | Ⲗ u => SN u
        end.
 Proof.
   induction 1 as [ [ x | u v | u ]  _ IH ]; auto.
@@ -331,10 +343,10 @@ Proof.
     * constructor; intros k Hk.
       refine (proj2 (IH (u@k) _)); auto.
   + constructor; intros k Hk.
-    apply (IH (λ k)); eauto.
+    apply (IH (Ⲗ k)); eauto.
 Qed.
 
-Fact term_beta_sn_app_inv a m : SN (a @* m) -> SN a /\ Forall SN m.
+Fact term_beta_sn_app_inv a m : SN (a @* m) → SN a ∧ Forall SN m.
 Proof.
   induction m as [ | ? ? IHm ] in a |- *; simpl; auto.
   intros [[]%term_beta_sn_inv ]%IHm; eauto.
@@ -349,47 +361,47 @@ Qed.
 (** This proof DOES NOT require computing the SN height of a and u⌈a⌉@*l 
      which gives a MAJOR SIMPLIFICATION over the previous version in the 
      coq-terms project, and also departs from the proof in Krivine's book *)
-Lemma term_beta_sn_app a u m : SN a -> SN (u⌈a⌉ @* m) -> SN (λ u @* a::m).
+Lemma term_beta_sn_app a u m : SN a → SN (u⌈a⌉ @* m) → SN (Ⲗ u @* a::m).
 Proof.
   (** We use the tailored Acc_rinv_lex_fun_rect induction principle *) 
   unfold SN; revert a u m;
   apply Acc_rinv_lex_fun_rect
     with (f := fun a u m => u⌈a⌉ @* m)
-         (g := fun a u m => λ u @* a::m);
+         (g := fun a u m => Ⲗ u @* a::m);
   fold SN;
   intros a u m H1 H2 IH1 IH2.
 
   (** Now we can proceed with the proof.
       First the Acc constructor and 
       then case analysis on the
-      possible successors of λu @* a::m 
+      possible successors of Ⲗu @* a::m 
       given by term_beta_redex_app_inv:
         + u⌈a⌉ @* m                  (Hm works)
-        + λv @* a::m with u -β-> v   (IH2 works)
-        + λu @* b::m with a -β-> b   (IH1 works)
-        + λu @* a::m' with m -β-> m'
+        + Ⲗv @* a::m with u -β-> v   (IH2 works)
+        + Ⲗu @* b::m with a -β-> b   (IH1 works)
+        + Ⲗu @* a::m' with m -β-> m'
              at one position in m    (IH2 works)
     *)
   constructor; fold SN; intros ? H%term_beta_redex_app_inv.
   destruct H as [ m | m v Hv | m b Hb | l v w r Hv ].
   + (** SN (u⌈a⌉ @* m) *)
     trivial.
-  + (** SN ((λv)@a @* m) *)
+  + (** SN ((Ⲗv)@a @* m) *)
     apply IH2.
     (** u -β-> v entails u⌈a⌉ @* m  -β+>  v⌈a⌉ @* m *)
     auto.
-  + (** SN ((λu)@b @* m) *)
+  + (** SN ((Ⲗu)@b @* m) *)
     apply IH1. 
     * trivial.
     * (** a -β-> b entails u⌈a⌉ @* m  -β*>  u⌈b⌉ @* m *)
       eauto.
-  + (** SN (λu @* a::l++w::r) *)
+  + (** SN (Ⲗu @* a::l++w::r) *)
     apply IH2.
     (** v -β-> w entails u⌈a⌉ @* l++v::r  -β->  u⌈a⌉ @* l++w::r *)
     eauto.
 Qed.
 
-Fact term_beta_sn_subst u f : SN (syn_subst u f) -> SN u.
+Fact term_beta_sn_subst u f : SN u⟪f⟫ → SN u.
 Proof.
   revert u; apply Acc_rinv_fun_rect; fold SN.
   intros u Hu IHu.
@@ -397,22 +409,23 @@ Proof.
   now apply IHu, term_beta_subst.
 Qed.
 
-Fact term_beta_sn_replace u a : SN (u⌈a⌉) -> SN u.
+Fact term_beta_sn_replace u a : SN (u⌈a⌉) → SN u.
 Proof. apply term_beta_sn_subst. Qed.
 
 Inductive ctx C : Prop :=
-  | ctx_intro :(forall a b, a -β-> b -> C⌈a⌉ -β-> C⌈b⌉)
-            -> (forall a u, term_neutral a 
-                       -> C⌈a⌉ -β-> u 
-                       -> (exists b, u = C⌈b⌉ /\ a -β-> b) 
-                       \/ (exists D, u = D⌈a⌉ /\ C -β-> D))
-            -> (forall D, C -β-> D -> ctx D)
-            -> ctx C.
+  | ctx_intro : (∀ a b, a -β-> b → C⌈a⌉ -β-> C⌈b⌉)
+              → (∀ a u, term_neutral a 
+                      → C⌈a⌉ -β-> u 
+                      → (∃b, u = C⌈b⌉ ∧ a -β-> b) 
+                      ∨ (∃D, u = D⌈a⌉ ∧ C -β-> D))
+              → (∀D, C -β-> D → ctx D)
+              → ctx C.
 
 Fact ctx_SN : ctx ⊆₁ SN.
 Proof. induction 1; constructor; eauto. Qed.
 
-Theorem term_app_ctx m : Forall SN m -> ctx (£0 @* map ↑ m).
+(* _ @* m is a ctx when m are all SN *)
+Theorem term_app_ctx m : Forall SN m → ctx (£0 @* map ↑ m).
 Proof.
   intros H%prod_list_Acc.
   induction H as [ m _ IHm ].
@@ -436,15 +449,15 @@ Proof.
     apply IHm; now constructor.
 Qed.
 
-Lemma term_beta_sn_ctx_sig a u (C : sig ctx) :
+Local Lemma term_beta_sn_ctx_sig a u (C : sig ctx) :
            SN a
-        -> SN ((proj1_sig C)⌈u⌈a⌉⌉) 
-        -> SN ((proj1_sig C)⌈λ u@a⌉).
+         → SN ((proj1_sig C)⌈u⌈a⌉⌉) 
+         → SN ((proj1_sig C)⌈Ⲗ u@a⌉).
 Proof.
   unfold SN; revert a u C.
   apply Acc_rinv_lex_fun_rect
     with (f := fun a u C => (proj1_sig C)⌈u⌈a⌉⌉)
-         (g := fun a u C => (proj1_sig C)⌈λ u @ a⌉);
+         (g := fun a u C => (proj1_sig C)⌈Ⲗ u @ a⌉);
   fold SN;
   intros a u (C & HC) H1 H2 IH1 IH2; simpl in *.
   constructor.
@@ -458,19 +471,18 @@ Proof.
   + apply (IH2 _ (exist _ D (HC3 _ HD))); simpl; eauto.
 Qed.
 
-Theorem term_beta_sn_ctx a u C : ctx C -> SN a -> SN (C⌈u⌈a⌉⌉) -> SN (C⌈λ u@a⌉).
+Theorem term_beta_sn_ctx C a u : ctx C → SN a → SN (C⌈u⌈a⌉⌉) → SN (C⌈Ⲗ u@a⌉).
 Proof. intros HC; apply term_beta_sn_ctx_sig with (C := exist _ C HC). Qed.
 
 (* An alternate, more modular proof *)
-Lemma term_beta_sn_app' a u m : SN a -> SN (u⌈a⌉ @* m) -> SN (λ u @* a::m).
+Lemma term_beta_sn_app' a u m : SN a → SN (u⌈a⌉ @* m) → SN (Ⲗ u @* a::m).
 Proof.
   intros H1 H2.
-  replace (λ u @* a::m) with ((£0 @* map ↑ m)⌈λ u @ a⌉).
-  + apply term_beta_sn_ctx; auto.
-    * apply term_app_ctx.
-      now apply term_beta_sn_app_inv in H2.
-    * now rewrite term_app_lift_replace.
+  replace (Ⲗ u @* a::m) with ((£0 @* map ↑ m)⌈Ⲗ u @ a⌉).
+  2: now rewrite term_app_lift_replace.
+  apply term_beta_sn_ctx; auto.
+  + apply term_app_ctx.
+    now apply term_beta_sn_app_inv in H2.
   + now rewrite term_app_lift_replace.
 Qed.
-  
 
