theories/syntax.v
@@ -7,37 +7,43 @@
 (*        Mozilla Public License Version 2.0, MPL-2.0         *)
 (**************************************************************)
 
-From Coq Require Import List.
+From Coq Require Import List Utf8.
 Import ListNotations.
 
 From SystemF Require Import utils.
 
 Set Implicit Arguments.
 
-Definition scons {X} x (f : nat -> X) n :=
+Definition scons {X} x (f : nat → X) n :=
   match n with
   | 0 => x
   | S n => f n
   end.
 
 #[global] Notation "x ∷ f" := (scons x f) (at level 45, right associativity).
+#[global] Notation "f ⋄ g" := (λ x,f (g x)) (at level 44, left associativity).
+
+#[global] Reserved Notation "u ⟪ f ⟫" (at level 1, left associativity, format "u ⟪ f ⟫").
+#[global] Reserved Notation "u ⟬ f ⟭" (at level 1, left associativity, format "u ⟬ f ⟭").
+(*#[global] Reserved Notation "'𝓥' u" (at level 2, format "𝓥 u"). *)
+#[global] Reserved Notation "u ⌈ v ⌉" (at level 50, format "u ⌈ v ⌉").
 
 Fixpoint list_pred l :=
   match l with
-  | [] => []
-  | 0::l => list_pred l
+  | []     => []
+  | 0::l   => list_pred l
   | S n::l => n::list_pred l
   end.
 
-Fact In_list_pred l n : S n ∈ l -> n ∈ list_pred l.
+Fact In_list_pred l n : S n ∈ l → n ∈ list_pred l.
 Proof. induction l as [ | [] ]; simpl; intros []; now eauto. Qed.
 
-Fact list_pred_In l n : n ∈ list_pred l -> S n ∈ l.
+Fact list_pred_In l n : n ∈ list_pred l → S n ∈ l.
 Proof. induction l as [ | [] ]; simpl; eauto; intros []; eauto. Qed.
 
 #[global] Hint Resolve In_list_pred list_pred_In : core.
 
-Fact In_list_pred_iff l n : n ∈ list_pred l <-> S n ∈ l.
+Fact In_list_pred_iff l n : n ∈ list_pred l ↔ S n ∈ l.
 Proof. split; auto. Qed.
 
 Fact list_pred_map_S l : list_pred (map S l) = l.
@@ -48,123 +54,128 @@ Proof. induction l as [ | [] ]; simpl; f_equal; auto. Qed.
 
 #[local] Hint Resolve in_or_app in_eq in_cons : core.
 
-Fact list_pred_mono l m : incl l m -> incl (list_pred l) (list_pred m).
+Fact list_pred_mono l m : incl l m → incl (list_pred l) (list_pred m).
 Proof. revert m; induction l as [ | [] ]; intros [ | [] ] ? ?; easy || eauto. Qed.
-
-#[global] Reserved Notation "u ⌈ v ⌉" (at level 50, format "u ⌈ v ⌉").
 
 Section syntax.
 
-  Implicit Type (b : bool).
+  Implicit Type (c : bool).
 
-  Inductive syntax b :=
-    | syn_var : nat -> syntax b
-    | syn_bin : syntax b -> syntax b -> syntax b
-    | syn_abs : syntax b -> syntax b.
+  Inductive syntax c :=
+    | syn_var : nat → syntax c                 (* Variables, binded or not *)
+    | syn_bop : syntax c → syntax c → syntax c (* Binary composition operator *)
+    | syn_bnd : syntax c → syntax c            (* Nameless de Bruijn binder *)
+    .
+
+  Notation "£" := syn_var.
+  Infix "⊘" := syn_bop (at level 45).
+  Notation Λ := syn_bnd.
 
   Arguments syn_var {_}.
 
-  Context {b : bool}.
+  Context {c : bool}.
 
-  Implicit Type (A : syntax b).
+  Implicit Type (u v : syntax c).
 
-  Fixpoint syn_vars A :=
-    match A with
-    | syn_var x => [x]
-    | syn_bin u v => syn_vars u ++ syn_vars v
-    | syn_abs u => list_pred (syn_vars u)
+  Fixpoint syn_vars u :=
+    match u with
+    | £ x   => [x]
+    | u ⊘ v => syn_vars u ++ syn_vars v
+    | Λ u   => list_pred (syn_vars u)
     end.
 
-  Fixpoint syn_ren A f : syntax b :=
-    match A with 
-    | syn_var n => syn_var (f n)
-    | syn_bin A B => syn_bin (syn_ren A f) (syn_ren B f)
-    | syn_abs A => syn_abs (syn_ren A (0∷fun n => S (f n)))
-    end.
+  Notation 𝓥 := (syn_vars).
 
-  Definition syn_lift A := syn_ren A S.
+  Fixpoint syn_ren u f : syntax c :=
+    match u with 
+    | £ n   => £ (f n)
+    | u ⊘ v => u⟬f⟭ ⊘ v⟬f⟭
+    | Λ u   => Λ u⟬0∷S⋄f⟭
+    end
+  where "u ⟬ f ⟭" := (syn_ren u f).
 
-  Fact syn_ren_ext A f g :
-        (forall x, x ∈ syn_vars A -> f x = g x)
-      -> syn_ren A f = syn_ren A g.
+  Definition syn_lift u := syn_ren u S.
+
+  Notation "↑" := syn_lift. (* x) (at level 1, format "↑ x"). *)
+
+  Fact syn_ren_ext u f g : (∀x, x ∈ 𝓥 u → f x = g x) → u⟬f⟭ = u⟬g⟭.
   Proof.
-    induction A as [ | | A IHA ] in f, g |- *; 
+    induction u as [ | | u IHu ] in f, g |- *; 
       simpl; intros Hfg; simpl; f_equal; eauto.
-    apply IHA; intros [] ?; simpl; auto.
+    apply IHu; intros [] ?; simpl; auto.
   Qed.
 
-  Fact syn_ren_vars A f : syn_vars (syn_ren A f) = map f (syn_vars A).
+  Fact syn_ren_vars u f : 𝓥 u⟬f⟭ = map f (𝓥 u).
   Proof.
-    induction A  as [ | | A IHA ] in f |- *; simpl; eauto.
+    induction u as [ | | u IHu ] in f |- *; simpl; eauto.
     + rewrite map_app; f_equal; auto.
-    + rewrite IHA; simpl; clear IHA.
-      induction (syn_vars A) as [ | [] ]; simpl; f_equal; eauto.
+    + rewrite IHu; simpl; clear IHu.
+      induction (syn_vars u) as [ | [] ]; simpl; f_equal; eauto.
   Qed.
 
-  Fact syn_lift_vars A : syn_vars (syn_lift A) = map S (syn_vars A).
+  Fact syn_lift_vars u : 𝓥 (↑u) = map S (𝓥 u).
   Proof. apply syn_ren_vars. Qed.
 
-  Fact syn_ren_id A : syn_ren A (fun x => x) = A.
+  Fact syn_ren_id u : u⟬λ x, x⟭ = u.
   Proof. 
-    induction A as [ | | A IHA ]; simpl; f_equal; eauto.
-    rewrite <- IHA at 2.
+    induction u as [ | | u IHu ]; simpl; f_equal; eauto.
+    rewrite <- IHu at 2.
     apply syn_ren_ext; now intros [].
   Qed.
 
-  Fact syn_ren_comp A f g : syn_ren (syn_ren A f) g = syn_ren A (fun n => g (f n)).
+  Fact syn_ren_comp u f g : u⟬f⟭⟬g⟭ = u⟬g⋄f⟭.
   Proof.
-    induction A as [ | | A IHA ] in f, g |- *;
+    induction u as [ | | u IHu ] in f, g |- *;
       simpl; f_equal; auto.
-    rewrite IHA.
+    rewrite IHu.
     apply syn_ren_ext; now intros [].
   Qed.
 
-  Fixpoint syn_subst A f :=
-    match A with 
-    | syn_var n => f n
-    | syn_bin A B => syn_bin (syn_subst A f) (syn_subst B f)
-    | syn_abs A => syn_abs (syn_subst A (syn_var 0∷fun n => syn_lift (f n)))
-    end.
+  Fixpoint syn_subst u f :=
+    match u with 
+    | £ n   => f n
+    | u ⊘ v => u⟪f⟫ ⊘ v⟪f⟫
+    | Λ u   => Λ u⟪£0∷↑⋄f⟫
+    end
+  where "u ⟪ f ⟫" := (syn_subst u f).
 
-  Fact syn_subst_ext A f g :
-        (forall x, x ∈ syn_vars A -> f x = g x)
-      -> syn_subst A f = syn_subst A g.
+  Fact syn_subst_ext u f g : (∀x, x ∈ 𝓥 u → f x = g x) → u⟪f⟫ = u⟪g⟫.
   Proof.
-    induction A as [ | | A IHA ] in f, g |- *;
+    induction u as [ | | u IHu ] in f, g |- *;
       simpl; intros Hfg; simpl; f_equal; eauto.
-    apply IHA.
+    apply IHu.
     intros [] ?; simpl; f_equal; eauto.
   Qed.
 
-  Fact syn_subst_vars A f : syn_vars (syn_subst A f) = flat_map (fun x => syn_vars (f x)) (syn_vars A).
+  Fact syn_subst_vars u f : 𝓥 u⟪f⟫ = flat_map (𝓥⋄f) (𝓥 u).
   Proof.
-    induction A  as [ | | A IHA ] in f |- *; eauto.
+    induction u as [ | | u IHu ] in f |- *; eauto.
     + simpl; now rewrite <- app_nil_end.
     + simpl; rewrite flat_map_app; f_equal; auto.
     + simpl syn_subst; simpl.
-      rewrite IHA; simpl; clear IHA.
-      induction (syn_vars A) as [ | [] ]; simpl; eauto.
-      now rewrite <- IHl, syn_lift_vars, list_pred_app, list_pred_map_S.
+      rewrite IHu; simpl; clear IHu.
+      induction (syn_vars u) as [ | [] l IH ]; simpl; eauto.
+      now rewrite <- IH, syn_lift_vars, list_pred_app, list_pred_map_S.
   Qed.
 
-  Fact syn_subst_id A : syn_subst A syn_var = A.
+  Fact syn_subst_id u : u⟪£⟫ = u.
   Proof.
-    induction A as [ | | A IHA ]; simpl; f_equal; eauto.
-    rewrite <- IHA at 2.
+    induction u as [ | | u IHu ]; simpl; f_equal; eauto.
+    rewrite <- IHu at 2.
     apply syn_subst_ext; now intros [].
   Qed.
 
-  Fact syn_subst_ren_comp A f g : syn_subst (syn_ren A f) g = syn_subst A (fun n => g (f n)).
+  Fact syn_subst_ren_comp u f g : u⟬f⟭⟪g⟫ = u⟪g⋄f⟫.
   Proof.
-    induction A as [ | | A IHA ] in f, g |- *; simpl; f_equal; auto.
-    rewrite IHA.
+    induction u as [ | | u IHu ] in f, g |- *; simpl; f_equal; auto.
+    rewrite IHu.
     apply syn_subst_ext; now intros [].
   Qed.
 
-  Fact syn_ren_subst_comp A f g : syn_ren (syn_subst A f) g = syn_subst A (fun n => syn_ren (f n) g).
+  Fact syn_ren_subst_comp u f g : u⟪f⟫⟬g⟭ = u⟪λ n, (f n)⟬g⟭⟫.
   Proof.
-    induction A as [ | | A IHA ] in f, g |- *; simpl; f_equal; auto.
-    rewrite IHA.
+    induction u as [ | | u IHu ] in f, g |- *; simpl; f_equal; auto.
+    rewrite IHu.
     apply syn_subst_ext.
     intros [] _; simpl; auto.
     unfold syn_lift.
@@ -172,10 +183,10 @@ Section syntax.
     apply syn_ren_ext; auto.
   Qed.
 
-  Fact syn_subst_comp A f g : syn_subst (syn_subst A f) g = syn_subst A (fun n => syn_subst (f n) g).
+  Fact syn_subst_comp u f g : u⟪f⟫⟪g⟫ = u⟪λ n, (f n)⟪g⟫⟫.
   Proof.
-    induction A as [ | | A IHA ] in f, g |- *; simpl; f_equal; auto.
-    rewrite IHA.
+    induction u as [ | | u IHu ] in f, g |- *; simpl; f_equal; auto.
+    rewrite IHu.
     apply syn_subst_ext.
     intros [] _; simpl; auto.
     unfold syn_lift.
@@ -183,40 +194,36 @@ Section syntax.
     apply syn_subst_ext; now intros [].
   Qed.
 
-  Fact syn_ren_eq_subst A f : syn_ren A f = syn_subst A (fun x => syn_var (f x)).
+  Fact syn_ren_eq_subst u f : u⟬f⟭ = u⟪£⋄f⟫.
   Proof.
-    induction A as [ | | A IHA ] in f |- *; simpl; f_equal; eauto.
-    rewrite IHA.
+    induction u as [ | | u IHu ] in f |- *; simpl; f_equal; eauto.
+    rewrite IHu.
     apply syn_subst_ext; now intros [].
   Qed.
 
-  Notation "£" := syn_var.
-  Notation "↑" := syn_lift.
-  Notation "u ⌈ v ⌉" := (syn_subst u (v∷£)).
+  Notation "u ⌈ v ⌉" := (u⟪v∷£⟫).
 
-  Fact syn_replace_vars A B x : x ∈ syn_vars (A⌈B⌉) -> x ∈ list_pred (syn_vars A) ++ syn_vars B.
+  Fact syn_replace_vars u v x : x ∈ 𝓥 (u⌈v⌉) → x ∈ list_pred (𝓥 u) ++ 𝓥 v.
   Proof.
     rewrite syn_subst_vars.
     intros ([|n] & H1 & H2)%in_flat_map; simpl in H2; eauto.
     destruct H2 as [ -> | [] ]; eauto.
   Qed.
 
-  Fact syn_ren_replace A B f : 
-       syn_ren (A⌈B⌉) f = (syn_ren A (0∷fun n => S (f n)))⌈syn_ren B f⌉.
+  Fact syn_ren_replace u v f : (u⌈v⌉)⟬f⟭ = u⟬0∷S⋄f⟭⌈v⟬f⟭⌉.
   Proof.
     rewrite syn_ren_subst_comp, syn_subst_ren_comp.
     apply syn_subst_ext; now intros [].
   Qed.
 
-  Fact syn_lift_replace A B : ↑A⌈B⌉ = A.
+  Fact syn_lift_replace u v : ↑u⌈v⌉ = u.
   Proof.
     unfold syn_lift.
     rewrite syn_subst_ren_comp; simpl.
     apply syn_subst_id.
   Qed.
 
-  Fact syn_subst_replace A B f : 
-       syn_subst (A⌈B⌉) f = (syn_subst A (£0∷fun n => ↑(f n)))⌈syn_subst B f⌉.
+  Fact syn_subst_replace u v f : (u⌈v⌉)⟪f⟫ = u⟪£0∷↑⋄f⟫⌈v⟪f⟫⌉.
   Proof.
     rewrite !syn_subst_comp.
     apply syn_subst_ext.
@@ -224,10 +231,10 @@ Section syntax.
     now rewrite syn_lift_replace.
   Qed.
 
-  Fact syn_replace_notfree A B C : ~ 0 ∈ syn_vars A -> A⌈B⌉ = A⌈C⌉.
+  Fact syn_replace_notfree u v w : ¬ 0 ∈ 𝓥 u → u⌈v⌉ = u⌈w⌉.
   Proof. intro; apply syn_subst_ext; intros [] ?; simpl; tauto. Qed. 
 
-  Fact syn_replace_lift A B : ~ 0 ∈ syn_vars A -> ↑(A⌈B⌉) = A.
+  Fact syn_replace_lift u v : ~ 0 ∈ 𝓥 u → ↑(u⌈v⌉) = u.
   Proof.
     intros H.
     unfold syn_lift.
@@ -237,18 +244,13 @@ Section syntax.
     intros []; simpl; tauto.
   Qed.
 
-  Fact syn_ren_var_eq_inv u f x : 
-         syn_var x = syn_ren u f -> exists y, u = syn_var y /\ x = f y.
+  Fact syn_ren_var_eq_inv u f x : £x = u⟬f⟭ → ∃y, u = £y ∧ x = f y.
   Proof. destruct u; simpl; try easy; inversion 1; eauto. Qed.
 
-  Fact syn_ren_bin_eq_inv u f p q : 
-         syn_bin p q = syn_ren u f 
-      -> exists p' q', u = syn_bin p' q' /\ p = syn_ren p' f /\ q = syn_ren q' f.
+  Fact syn_ren_bin_eq_inv u f p q : p ⊘ q = u⟬f⟭ → ∃p' q', u = p' ⊘ q' ∧ p = p'⟬f⟭ ∧ q = q'⟬f⟭.
   Proof. destruct u; try easy; simpl; inversion 1; eauto. Qed.
 
-  Fact syn_ren_abs_eq_inv u f v : 
-         syn_abs v = syn_ren u f 
-      -> exists u', u = syn_abs u' /\ v = syn_ren u' (0∷(fun n  => S (f n))).
+  Fact syn_ren_abs_eq_inv u f v : Λ v = u⟬f⟭ → ∃u', u = Λ u' ∧ v = u'⟬0∷S⋄f⟭.
   Proof. destruct u; try easy; simpl; inversion 1; eauto. Qed.
 
 End syntax.
@@ -256,22 +258,27 @@ End syntax.
 Notation type := (syntax false).
 Notation term := (syntax true).
 
+Notation 𝓥 := (@syn_vars _).
+
 Notation "£" := (@syn_var _).
 Notation "↑" := (@syn_lift _).
+
+Notation "u ⟬ f ⟭" := (syn_ren u f).
+Notation "u ⟪ f ⟫" := (syn_subst u f).
 Notation "u ⌈ v ⌉" := (@syn_subst _ u (v∷£)).
 Notation "⇑ Γ" := (fun x => ↑(Γ x)) (at level 1, format "⇑ Γ").
 
-Notation "A ⇨ B" := (@syn_bin _ A B) (at level 60, only parsing).
-Notation "∀ A" := (@syn_abs _ A) (at level 60, only parsing).
+Notation "A ⇨ B" := (@syn_bop _ A B) (at level 60, only parsing).
+Notation "∇ A" := (@syn_bnd _ A) (at level 60, only parsing).
 
-Notation "A ⇨ B" := (@syn_bin false A B) (at level 60, format "A ⇨ B", only printing).
-Notation "∀ A" := (@syn_abs false A) (at level 60, format "∀ A", only printing).
+Notation "A ⇨ B" := (@syn_bop false A B) (at level 60, format "A ⇨ B", only printing).
+Notation "∇ A" := (@syn_bnd false A) (at level 60, format "∇ A", only printing).
 
-Notation "u @ v" := (@syn_bin _ u v) (at level 50, only parsing).
-Notation "'λ' u" := (@syn_abs _ u) (at level 50, only parsing).
+Notation "u @ v" := (@syn_bop _ u v) (at level 50, only parsing).
+Notation "'Ⲗ' u" := (@syn_bnd _ u) (at level 50, only parsing).
 
-Notation "u @ v" := (@syn_bin true u v) (at level 50, format "u @ v", only printing).
-Notation "'λ' u" := (@syn_abs true u) (at level 50, format "λ u", only printing).
+Notation "u @ v" := (@syn_bop true u v) (at level 50, format "u @ v", only printing).
+Notation "'Ⲗ' u" := (@syn_bnd true u) (at level 50, format "Ⲗ u", only printing).
 
 #[global] Reserved Notation "f '@*' l" (at level 61, left associativity).
 
@@ -288,7 +295,7 @@ Proof. induction l in u |- *; simpl; auto. Qed.
 Fact term_app_snoc u l v : u @* (l++[v]) = (u @* l) @ v.
 Proof. now rewrite term_app_comp. Qed.
 
-Fact term_app_vars u l : syn_vars (u @* l) = flat_map syn_vars (u::l).
+Fact term_app_vars u l : 𝓥 (u @* l) = flat_map 𝓥 (u::l).
 Proof.
   induction l as [ | a l IHl ] in u |- *; simpl.
   + now rewrite <- app_nil_end.
